theories/language/tactics.v
@@ -20,20 +20,24 @@ Ltac reshape_expr e tac :=
         | _ =>
             fail
         end
-    | App ?e (Val ?v) =>
-        add_ectxi (CtxAppL v) vs K e
+    | App ?e1 (Val ?v2) =>
+        add_ectxi (CtxAppL v2) vs K e1
     | App ?e1 ?e2 =>
         add_ectxi (CtxAppR e1) vs K e2
     | Unop ?op ?e =>
         add_ectxi (CtxUnop op) vs K e
-    | Binop ?op ?e (Val ?v) =>
-        add_ectxi (CtxBinopL op v) vs K e
+    | Binop ?op ?e1 (Val ?v2) =>
+        add_ectxi (CtxBinopL op v2) vs K e1
     | Binop ?op ?e1 ?e2 =>
         add_ectxi (CtxBinopR op e1) vs K e2
+    | Equal ?e1 (Val ?v2) =>
+        add_ectxi (CtxEqualL v2) vs K e1
+    | Equal ?e1 ?e2 =>
+        add_ectxi (CtxEqualR e1) vs K e2
     | If ?e0 ?e1 ?e2 =>
         add_ectxi (CtxIf e1 e2) vs K e0
-    | Pair ?e (Val ?v) =>
-        add_ectxi (CtxPairL v) vs K e
+    | Pair ?e1 (Val ?v2) =>
+        add_ectxi (CtxPairL v2) vs K e1
     | Pair ?e1 ?e2 =>
         add_ectxi (CtxPairR e1) vs K e2
     | Fst ?e =>
@@ -46,14 +50,14 @@ Ltac reshape_expr e tac :=
         add_ectxi CtxInjr vs K e
     | Case ?e0 ?e1 ?e2 =>
         add_ectxi (CtxCase e1 e2) vs K e0
-    | Alloc ?e (Val ?v) =>
-        add_ectxi (CtxAllocL v) vs K e
+    | Alloc ?e1 (Val ?v2) =>
+        add_ectxi (CtxAllocL v2) vs K e1
     | Alloc ?e1 ?e2 =>
         add_ectxi (CtxAllocR e1) vs K e2
     | Load ?e =>
         add_ectxi CtxLoad vs K e
-    | Store ?e (Val ?v) =>
-        add_ectxi (CtxStoreL v) vs K e
+    | Store ?e1 (Val ?v2) =>
+        add_ectxi (CtxStoreL v2) vs K e1
     | Store ?e1 ?e2 =>
         add_ectxi (CtxStoreR e1) vs K e2
     | Cas ?e0 (Val ?v1) (Val ?v2) =>
@@ -62,16 +66,16 @@ Ltac reshape_expr e tac :=
         add_ectxi (CtxCasM e0 v2) vs K e1
     | Cas ?e0 ?e1 ?e2 =>
         add_ectxi (CtxCasR e0 e1) vs K e2
-    | Faa ?e (Val ?v) =>
-        add_ectxi (CtxFaaL v) vs K e
+    | Faa ?e1 (Val ?v2) =>
+        add_ectxi (CtxFaaL v2) vs K e1
     | Faa ?e1 ?e2 =>
         add_ectxi (CtxFaaR e1) vs K e2
-    | Resolve ?ex (Val ?v1) (Val ?v2) =>
-        go K ((v1,v2) :: vs) ex
-    | Resolve ?ex ?e1 (Val ?v2) =>
-        add_ectxi (CtxResolveM ex v2) vs K e1
-    | Resolve ?ex ?e1 ?e2 =>
-        add_ectxi (CtxResolveR ex e1) vs K e2
+    | Resolve ?e0 (Val ?v1) (Val ?v2) =>
+        go K ((v1, v2) :: vs) e0
+    | Resolve ?e0 ?e1 (Val ?v2) =>
+        add_ectxi (CtxResolveM e0 v2) vs K e1
+    | Resolve ?e0 ?e1 ?e2 =>
+        add_ectxi (CtxResolveR e0 e1) vs K e2
     end
   with add_ectxi k vs K e :=
     lazymatch vs with
@@ -95,16 +99,25 @@ Ltac invert_head_step :=
   end.
 
 #[global] Hint Extern 0 (
+  val_physical _
+) =>
+  apply val_not_literal_physical
+: zebre.
+#[global] Hint Extern 0 (
+  val_physically_distinct _ _
+) =>
+  apply val_not_literal_physically_distinct
+: zebre.
+
+#[global] Hint Extern 0 (
   head_reducible _ _
 ) =>
-  eexists _, _, _, _;
-  simpl
+  do 4 eexists; simpl
 : zebre.
 #[global] Hint Extern 0 (
   head_reducible_no_obs _ _
 ) =>
-  eexists _, _, _;
-  simpl
+  do 3 eexists; simpl
 : zebre.
 
 #[global] Hint Extern 1 (
@@ -113,13 +126,29 @@ Ltac invert_head_step :=
   econstructor
 : zebre.
 #[global] Hint Extern 0 (
-  head_step (Cas _ _ _) _ _ _ _ _
+  head_step (Equal _ _) _ _ _ _ _
 ) =>
-  eapply head_step_cas
+  eapply head_step_equal_fail
+: zebre.
+#[global] Hint Extern 0 (
+  head_step (Equal _ _) _ _ _ _ _
+) =>
+  eapply head_step_equal_suc
 : zebre.
 #[global] Hint Extern 0 (
   head_step (Alloc _ _) _ _ _ _ _
-) => apply head_step_alloc'
+) =>
+  apply head_step_alloc'
+: zebre.
+#[global] Hint Extern 0 (
+  head_step (Cas _ _ _) _ _ _ _ _
+) =>
+  eapply head_step_cas_fail
+: zebre.
+#[global] Hint Extern 0 (
+  head_step (Cas _ _ _) _ _ _ _ _
+) =>
+  eapply head_step_cas_suc
 : zebre.
 #[global] Hint Extern 0 (
   head_step Proph _ _ _ _ _
